AES-XTS encrypt (any input length) spec. To be tested

arm/proofs/aes_xts_encrypt_spec.ml
@@ -1,3 +1,4 @@
+needs "arm/proofs/base.ml";;
 needs "arm/proofs/aes_encrypt_spec.ml";;
 (*
 AES-256-XTS Encryption Algorithm for One Block
@@ -12,7 +13,7 @@ i is the value of the 128-bit tweak (see 5.1)
 j is the sequential number of the 128-bit block inside the data unit
 C is the block of 128 bits of ciphertext resulting from the operation
 
-T := AES-enc(Key2 , i) XOR α^j
+T := AES-enc(Key2 , i) MUL α^j
 PP := P XOR T
 CC := AES-enc(Key1 , PP)
 C := CC XOR T
@@ -77,31 +78,195 @@ let tweak_key_schedule = new_definition `tweak_key_schedule:int128 list =
   ; word 0x4E12BD760FE7F086777A3655FF5B9B4D
   ; word 0x70ADE5BA1B23A3A2807BD0C6E50F5D04
   ]`;;
+
 (*
-let AES_XTS_ENC_HELPER_CONV =
-    PRINT_TERM_CONV THENC
-  REWR_CONV aes256_xts_encrypt_one_block THENC
-    PRINT_TERM_CONV THENC
-  REWRITE_CONV [aes256_encrypt; data_key_schedule; tweak_key_schedule] THENC
-    PRINT_TERM_CONV THENC
-  REWRITE_CONV EL_15_128_CLAUSES THENC
-(*  PRINT_TERM_CONV THENC *)
-  REPEATC let_CONV THENC
-  DEPTH_CONV (WORD_RED_CONV ORELSEC NUM_RED_CONV) THENC
-  DEPTH_CONV AESENC_REDUCE_CONV (*THENC
-  AES_SHIFT_ROWS_CONV THENC
-  AES_SUB_BYTES_CONV THENC
-  PRINT_TERM_CONV THENC
-  DEPTH_CONV (WORD_RED_CONV ORELSEC NUM_RED_CONV)
-  *)
-  ;;
+AES-256-XTS Encryption Algorithm for Any Input Length
+Based on IEEE 1619-2007 Standard
+
+This specification implements the complete AES-XTS encryption algorithm
+as described in IEEE 1619-2007, Section 5.3, supporting arbitrary input lengths.
+
+Key components:
+- Key = Key1 (256-bit data key) || Key2 (256-bit tweak key)
+- P is the plaintext of arbitrary length (≥ 128 bits)
+- i is the value of the 128-bit tweak
+- C is the resulting ciphertext
+
+The algorithm processes data in 128-bit blocks with special handling for
+the final partial block (if any) using ciphertext stealing.
+
+For each complete block j:
+  T_j := AES-enc(Key2, i) MUL α^j
+  PP_j := P_j XOR T_j
+  CC_j := AES-enc(Key1, PP_j)
+  C_j := CC_j XOR T_j
+
+Where α is the primitive element in GF(2^128) and MUL denotes multiplication
+in the Galois field.
+
+For partial final blocks, ciphertext stealing is used as per Section 5.3.2.
 *)
-let AES_XTS_ENC_HELPER_CONV =
+
+(*****************************************)
+(* AES-XTS encryption full *)
+
+(* Note: the implementation sequences the calculation of the tweak for each block,
+   however, the specification will calculate the tweak from the very beginning for each block.
+   We write the specification in the sequenced version for proof simplicity. *)
+
+(* Helper functions derived from Amanda's code:
+   https://github.com/amanda-zx/s2n-bignum/blob/sha512/arm/sha512/sha512_specs.ml#L360 *)
+
+(* XTS tweak initialization - encrypt the IV with key2 *)
+(* TODO: put it in a common place to be used with decrypt
+     Start *)
+let xts_init_tweak = new_definition
+  `xts_init_tweak (iv:int128) (key_schedule:int128 list) =
+     aes256_encrypt iv key_schedule`;;
+
+let bytes_to_int128 = define
+  `bytes_to_int128 (bs : byte list) : int128 =
+     word_join
+       (word_join
+         (word_join
+           (word_join (EL 15 bs) (EL 14 bs) : int16)
+           (word_join (EL 13 bs) (EL 12 bs) : int16) : int32)
+         (word_join
+           (word_join (EL 11 bs) (EL 10 bs) : int16)
+           (word_join (EL 9 bs) (EL 8 bs) : int16) : int32) : int64)
+       (word_join
+         (word_join
+           (word_join (EL 7 bs) (EL 6 bs) : int16)
+           (word_join (EL 5 bs) (EL 4 bs) : int16) : int32)
+         (word_join
+           (word_join (EL 3 bs) (EL 2 bs) : int16)
+           (word_join (EL 1 bs) (EL 0 bs) : int16) : int32) : int64)`;;
+
+let int128_to_bytes = define
+  `int128_to_bytes (w : int128) : byte list =
+     [word_subword w (0, 8); word_subword w (8, 8); word_subword w (16, 8); word_subword w (24, 8);
+      word_subword w (32, 8); word_subword w (40, 8); word_subword w (48, 8); word_subword w (56, 8);
+      word_subword w (64, 8); word_subword w (72, 8); word_subword w (80, 8); word_subword w (88, 8);
+      word_subword w (96, 8); word_subword w (104, 8); word_subword w (112, 8); word_subword w (120, 8)]`;;
+
+(* Multiplication by the primitive element \alpha in GF(2^128) *)
+let GF_128_mult_by_primitive = new_definition
+  `GF_128_mult_by_primitive (tweak:(128)word) =
+     let shifted = word_shl tweak 1 in
+     let mask = word_ishr tweak 127 in
+     word_xor (word_and mask (word 0x87)) shifted`;;
+
+let FST3 = define `FST3 (x:a#b#c) = FST x`;;
+let SND3 = define `SND3 (x:a#b#c) = FST (SND x)`;;
+let THD3 = define `THD3 (x:a#b#c) = SND (SND x)`;;
+
+(* TODO: put it in a common place to be used with decrypt
+     End *)
+
+(* AES-XTS encryption round function *)
+let aes256_xts_encrypt_round = new_definition
+  `aes256_xts_encrypt_round (P:int128) (tk:int128) (key_schedule:int128 list) =
+     let PP = word_xor P tk in
+     let CC = aes256_encrypt PP key_schedule in
+     word_xor CC tk`;;
+
+(* Single block AES-XTS encryption *)
+let aes256_xts_encrypt_1block = new_definition
+  `aes256_xts_encrypt_1block (P:int128) (iv:int128) (key1:int128 list) (key2:int128 list) =
+     let tk = xts_init_tweak iv key2 in
+     aes256_xts_encrypt_round P tk key1`;;
+
+(* Recursive encryption function for multiple blocks *)
+let eth = prove_general_recursive_function_exists
+  `?aes256_xts_encrypt_rec.
+     ! (i:num) (m:num) (P:byte list) (iv:int128) (key1:int128 list) (key2:int128 list).
+       aes256_xts_encrypt_rec i m P iv key1 key2 : (byte list)#int128#num =
+         if m < i then ([], iv, i)
+         else
+           let current_block = bytes_to_int128 (SUB_LIST (i * 16, 16) P) in
+           let curr = int128_to_bytes (aes256_xts_encrypt_round current_block iv key1) in
+           let iv = GF_128_mult_by_primitive iv in
+           let res = aes256_xts_encrypt_rec (i + 1) m P iv key1 key2 in
+           (APPEND curr (FST3 res), SND3 res, THD3 res)`;;
+
+let wfth = prove(hd(hyp eth),
+  EXISTS_TAC `MEASURE (\(i:num,m:num,P:byte list,iv:int128,key1:int128 list,key2:int128 list). (m + 1) - i)` THEN
+  REWRITE_TAC[WF_MEASURE; MEASURE] THEN ARITH_TAC);;
+
+let exists_lemma = PROVE_HYP wfth eth;;
+
+(* Note: results are stored in LSByte to MSByte *)
+let aes256_xts_encrypt_rec = new_specification ["aes256_xts_encrypt_rec"] exists_lemma;;
+
+(* Cipher stealing for encryption (note: encryption cipher stealing is different from decryption) *)
+let cipher_stealing_encrypt = new_definition
+  `cipher_stealing_encrypt (block:int128) (tail:int128) (tail_len:num) (iv:int128) (key1:int128 list) : int128#int128 =
+     let CC = aes256_xts_encrypt_round block iv key1 in
+     let Cm = word_subword CC (0,  tail_len * 8) in
+     let CP = word_subword CC (tail_len * 8, (16 - tail_len) * 8) in
+     let PP = word_join (word_subword tail (0, tail_len * 8)) CP in
+     let iv_last = GF_128_mult_by_primitive iv in
+     let Cm1 = aes256_xts_encrypt_round PP iv_last key1 in
+     (Cm1, (word_zx Cm))`;;
+
+(* Encryption tail handling - either single block or cipher stealing *)
+let aes256_xts_encrypt_tail = new_definition
+  `aes256_xts_encrypt_tail (i:num) (m:num) (tail:num) (P:byte list) (iv:int128) (key1:int128 list) (key2:int128 list) : byte list =
+     let Pm1 = bytes_to_int128 (SUB_LIST (i * 16, 16) P) in
+     if tail = 0 then
+       int128_to_bytes (aes256_xts_encrypt_round Pm1 iv key1)
+     else
+       let padded_tail = APPEND (SUB_LIST ((i + 1) * 16, tail) P) (REPLICATE (16 - tail) (word 0)) in
+       let Ptail = bytes_to_int128 padded_tail in
+       let res_cs = cipher_stealing_encrypt Pm1 Ptail tail iv key1 in
+       let Cm1 = int128_to_bytes (FST res_cs) in
+       let Ctail = SUB_LIST (0, tail) (int128_to_bytes (SND res_cs)) in
+       APPEND Cm1 Ctail`;;
+
+(* The main encryption function *)
+(* Note: the specification does not handle the case of len < 16, which is
+   handled in the implementation. *)
+(* AES256-XTS assumes there is at least one block in input *)
+(*
+  P: Input plaintext represented as a byte list
+  len: Byte length of P
+  iv: Initialization vector (tweak) as an int128
+  key1: Key schedule for AES-256 encryption
+  key2: Key schedule for AES-256 encryption for the tweak
+  C_error: Error output ciphertext in case of invalid input length
+  return: Output ciphertext as a byte list
+  When input len < 16, the function returns C_error,
+  which will be the initial value stored in output address.
+*)
+(* TODO: Challenge lemma: proving that the output is of same length as input *)
+(* TODO: Double check if NIST spec talks about the error case len < 16 *)
+(* TODO: Double check the pseudo code in the spec for tweak calculation in ANEX c *)
+let aes256_xts_encrypt = new_definition
+  `aes256_xts_encrypt
+     (P:byte list) (len:num) (iv:int128) (key1:int128 list) (key2:int128 list) (C_error:byte list) : byte list =
+     if len < 16 then
+       C_error
+     else
+       let tail = len MOD 16 in
+       let m = (len - tail) DIV 16 in
+       let i = 0 in
+       let iv = xts_init_tweak iv key2 in
+       if m < 2 then
+         aes256_xts_encrypt_tail i m tail P iv key1 key2
+       else
+         let res = aes256_xts_encrypt_rec 0 (m - 2) P iv key1 key2 in
+         let Ctail = aes256_xts_encrypt_tail (THD3 res) m tail P (SND3 res) key1 key2 in
+         APPEND (FST3 res) Ctail`;;
+
+(****)
+(* Conversions and test vectors *)
+let AES_XTS_ENC_1BLK_HELPER_CONV =
 (*    PRINT_TERM_CONV THENC *)
-  REWR_CONV aes256_xts_encrypt_one_block THENC
-(*    PRINT_TERM_CONV THENC*)
+  REWR_CONV aes256_xts_encrypt_1block THENC
+    PRINT_TERM_CONV THENC
   REWRITE_CONV [data_key_schedule; tweak_key_schedule] THENC
-(*  PRINT_TERM_CONV THENC *)
+   (* PRINT_TERM_CONV THENC *)
+  REWRITE_CONV [xts_init_tweak; aes256_xts_encrypt_round] THENC
   REPEATC let_CONV THENC
   DEPTH_CONV (WORD_RED_CONV ORELSEC NUM_RED_CONV) THENC
   DEPTH_CONV AESENC_HELPER_CONV THENC
@@ -109,13 +274,24 @@ let AES_XTS_ENC_HELPER_CONV =
   ;;
 
 (*
-(* Takes about a 100 sec on M3 *)
-let tmp_xts = AES_XTS_ENC_HELPER_CONV
-  `aes256_xts_encrypt_one_block
+(* Proven in about 100 sec on M3 *)
+time prove(`aes256_xts_encrypt_1block
+        (word 0x0F0E0D0C0B0A09080706050403020100)
+        (word 0x000000000000000000000000000000FF)
+        data_key_schedule
+        tweak_key_schedule
+      = word 0x9BCF70E3996C83E48603772F103A3B1C`,  (* expected result in little endian *)
+      CONV_TAC(LAND_CONV AES_XTS_ENC_1BLK_HELPER_CONV)
+      THEN REFL_TAC
+    );;
+*)
+(*
+let tmp_xts = AES_XTS_ENC_1BLK_HELPER_CONV
+  `aes256_xts_encrypt_1block
     (word 0x0F0E0D0C0B0A09080706050403020100)
+    (word 0x000000000000000000000000000000FF)
     data_key_schedule
     tweak_key_schedule
-    (word 0x000000000000000000000000000000FF)
   `;;
 
 prove(list_mk_comb (`(=):((128)word->(128)word->bool)`,
@@ -124,14 +300,125 @@ prove(list_mk_comb (`(=):((128)word->(128)word->bool)`,
 *)
 
 (*
-(* Takes about a 100 sec on M3 *)
-time prove(`aes256_xts_encrypt_one_block
-        (word 0x0F0E0D0C0B0A09080706050403020100)
-        data_key_schedule
-        tweak_key_schedule
-        (word 0x000000000000000000000000000000FF)
-      = word 0x9BCF70E3996C83E48603772F103A3B1C`,  (* expected result in little endian *)
-      CONV_TAC(LAND_CONV AES_XTS_ENC_HELPER_CONV)
-      THEN REFL_TAC
-       );;
+  Two-block test vector (same key and tweak as single block)
+  Plaintext:  000102030405060708090a0b0c0d0e0f101112131415161718191a1b1c1d1e1f
+  Data Key:   2718281828459045235360287471352662497757247093699959574966967627
+  Tweak Key:  3141592653589793238462643383279502884197169399375105820974944592
+  Tweak:      FF000000000000000000000000000000
+  Ciphertext: 1C3B3A102F770386E4836C99E370CF9BEA00803F5E482357A4AE12D414A3E63B
+  Plaintext (reversed):  1F1E1D1C1B1A191817161514131211100F0E0D0C0B0A09080706050403020100
+  Ciphertext (reversed): 3BE6A314D412AEA45723485E3F8000EA9BCF70E3996C83E48603772F103A3B1C
 *)
+
+(* Convert reversed plaintext and ciphertext to byte lists using int128_to_bytes *)
+let plaintext = new_definition
+  `plaintext =
+   int128_to_bytes (word 0x1F1E1D1C1B1A191817161514131211100F0E0D0C0B0A09080706050403020100)`;;
+
+let ciphertext = new_definition
+  `ciphertext =
+   int128_to_bytes (word 0x3BE6A314D412AEA45723485E3F8000EA9BCF70E3996C83E48603772F103A3B1C)`;;
+
+let cerr = new_definition
+  `cerr =
+   int128_to_bytes (word 0x0)`;;
+
+(* Generated by Cline but not needed
+(* Two-block plaintext for testing *)
+let two_block_plaintext = new_definition
+  `two_block_plaintext =
+   APPEND (int128_to_bytes (word 0x0F0E0D0C0B0A09080706050403020100))
+          (int128_to_bytes (word 0x1F1E1D1C1B1A19181716151413121110))`;;
+*)
+
+(* This was generated by Cline, to review *)
+(* Conversion for aes256_xts_encrypt using the byte lists *)
+let AES_XTS_ENC_HELPER_CONV =
+(*    PRINT_TERM_CONV THENC *)
+  REWR_CONV aes256_xts_encrypt THENC
+    PRINT_TERM_CONV THENC
+  REWRITE_CONV [data_key_schedule; tweak_key_schedule; plaintext; ciphertext; C_err] THENC
+   (* PRINT_TERM_CONV THENC *)
+  REWRITE_CONV [xts_init_tweak; aes256_xts_encrypt_round; aes256_xts_encrypt_tail;
+                aes256_xts_encrypt_rec; cipher_stealing_encrypt] THENC
+  REWRITE_CONV [int128_to_bytes; bytes_to_int128; SUB_LIST; APPEND; EL] THENC
+  REPEATC let_CONV THENC
+  DEPTH_CONV (WORD_RED_CONV ORELSEC NUM_RED_CONV) THENC
+  DEPTH_CONV AESENC_HELPER_CONV THENC
+  DEPTH_CONV (WORD_RED_CONV ORELSEC NUM_RED_CONV)
+  ;;
+
+  let tmp_xts_enc = AES_XTS_ENC_HELPER_CONV
+    `aes256_xts_encrypt plaintext 32 (word 0x000000000000000000000000000000FF)
+            data_key_schedule
+            tweak_key_schedule C_error
+    `;;
+(*****************************************)
+(* Test key schedules from the decryption spec *)
+
+let KEY1 = new_definition `KEY1:int128 list =
+  [ word 0xc70a951e84370d1836bdd387607e94e5
+  ; word 0x7ead95d6f74bf6b3103340cce21b473d
+  ; word 0x298c296cdf3241d53d0757ddbebda060
+  ; word 0x89e66365e778b67ff22807f1cdc91c8f
+  ; word 0xf6be68b9e235160883baf7bd2340b902
+  ; word 0x6e9ed51a1550b18e3fe11b7e185c513e
+  ; word 0x148b7eb1618fe1b5a0fa4ebf336ae76e
+  ; word 0x7bce64942ab1aaf027bd4a40982968cd
+  ; word 0x75049f04c175af0a9390a9d1d91a6526
+  ; word 0x517fce640d0ce0b0bf94228de7e3085d
+  ; word 0xb471300e52e506db4a8accf7a81afe26
+  ; word 0x5c732ed4b298c23d58772ad0be94ce31
+  ; word 0xe69436d5186fca2ce29032d11463c620
+  ; word 0xeeebece9eaefe8ede6e3e4e1e2e7e0e5
+  ; word 0xf0f1f2f3f4f5f6f7f8f9fafbfcfdfeff
+  ]`;;
+
+let KEY2 = new_definition `KEY2:int128 list =
+  [ word 0xb0b1b2b3b4b5b6b7b8b9babbbcbdbebf
+  ; word 0xa0a1a2a3a4a5a6a7a8a9aaabacadaeaf
+  ; word 0x0ae0323bba5180880ee4363fb65d8c84
+  ; word 0x67e123e2c740814163e527e6cb4c8d4d
+  ; word 0x908df02c9a6dc217203c429f2ed874a0
+  ; word 0x685584790fb4a79bc8f426daab11013c
+  ; word 0xb241f85f22cc0873b8a1ca64989d88fb
+  ; word 0x338745cb5bd2c1b2546666299c9240f3
+  ; word 0xaf72a5d51d335d8a3fff55f9875e9f9d
+  ; word 0xd9e1a4a0ea66e16bb1b420d9e5d246f0
+  ; word 0xead5ca6245a76fb75894323d676b67c4
+  ; word 0xe0e257483903f3e8d365128362d1325a
+  ; word 0xc26c685728b9a2356d1ecd82358affbf
+  ; word 0x4d05c122ade7966a94e4658247817701
+  ; word 0x21a29367e3cefb30cb775905a6699487
+  ]`;;
+
+(*****************************************)
+(* Conversions *)
+
+let plaintext = new_definition
+  `[word 0x0f; word 0x0e; word 0x0d; word 0x0c
+  ; word 0x0b; word 0x0a; word 0x09; word 0x08
+  ; word 0x07; word 0x06; word 0x05; word 0x04
+  ; word 0x03; word 0x02; word 0x01; word 0x00] : byte list`;;
+
+let iv = new_definition
+  `(word 0x0000000000000000000000123456789a) : int128`;;
+
+let C_error = new_definition
+  `[ word 0; word 0; word 0; word 0
+  ; word 0; word 0; word 0; word 0
+  ; word 0; word 0; word 0; word 0
+  ; word 0; word 0; word 0; word 0] : byte list`;;
+
+let ciphertext = new_definition
+  `[word 0xc3; word 0x0c; word 0xa8; word 0xf2
+  ; word 0xed; word 0x57; word 0x30; word 0x7e
+  ; word 0xdc; word 0x87; word 0xe5; word 0x44
+  ; word 0x86; word 0x7a; word 0xc8; word 0x88] : byte list`;;
+
+let rw = Compute.bool_compset();;
+word_compute_add_convs rw;;
+num_compute_add_convs rw;;
+Compute.add_thms [aes256_xts_encrypt;KEY1;KEY2;plaintext;iv;C_error;ciphertext] rw;;
+let my_conv = Compute.WEAK_CBV_CONV rw;;
+my_conv `aes256_xts_encrypt P 16 iv KEY1 KEY2 C_error`;;
